Velvet/Examples/SimplestSort.lean
@@ -19,13 +19,13 @@ for i in 0..n do
 ```
 -/
 
-@[grind, simp]
+@[grind]
 public def cnt (arr : Array Int) (x : Int) : Nat := arr.toList.count x
 
-@[grind, simp]
+@[grind]
 public def sameElems (a b : Array Int) : Prop := ∀ x, cnt a x = cnt b x
 
-@[grind, simp]
+@[grind]
 public def SortedUpTo (arr : Array Int) (n : Nat) : Prop :=
   ∀ i j, i ≤ j → j < n → arr[i]! ≤ arr[j]!
 
